WIP

RV32I/BitNotations.lean
@@ -4,19 +4,23 @@ import Mathlib.Data.Fin.VecNotation
 #check decidableGetElem?
 #check Matrix.vecCons
 #check tacticGet_elem_tactic_trivial
+#check Lean.RArray
+
+/-
+https://github.com/leanprover/lean4-nightly/commit/f6c5aed7ef6758f8357d5cee9c509ebc64c4e45a#diff-b4b5e504e6b8f2b07aa8846220cc5721760a789c37ddf9a802b8c9d9a31542b9R6
+-/
 
 /-- Notation for splitting bit vectors. `x#[m, n, k]`  -/
 syntax:max term noWs "#[" withoutPosition(term,+) "]" : term
 macro_rules
-  | `($x#[$ns:term,*, $m:term]) => do
-    let rec genProd (ns : List Lean.Term) : Lean.MacroM (Lean.Term × Lean.Term) := do
-      match ns with
-      | [] => return ⟨← `(BitVec.extractLsb' 0 $m $x), m⟩
-      | n::ns =>
+  | `($x#[$ns:term,*, $m:term]) =>
+    let rec genProd : List Lean.Term → Lean.MacroM (Lean.Term × Lean.Term)
+      | [] => return ⟨← ``(BitVec.extractLsb' 0 $m $x), m⟩
+      | n::ns => do
         let ⟨xs, sum⟩ ← genProd ns
-        return ⟨← `(Prod.mk (BitVec.extractLsb' $sum $n $x) $xs), ← `($n + $sum)⟩
+        return ⟨← ``(Prod.mk (BitVec.extractLsb' $sum $n $x) $xs), ← `($n + $sum)⟩
     return (← genProd ns.getElems.toList).1
-  | `($x#[$n:term]) => `(($x : BitVec $n))
+  | `($x#[$n:term]) => ``(($x : BitVec $n))
 
 #check_failure (0#7)#[1]
 #check_failure (0#7)#[10]
@@ -32,3 +36,55 @@ example : (0b001_01_01#7)#[3, 2, 2] = (1#3, 1#2, 1#2) := rfl
 example : (1#7)#[3, 2, 2] =
     ((1#7).extractLsb' 4 3, (1#7).extractLsb' 2 2, (1#7).extractLsb' 0 2) :=
   rfl
+
+-- def extractLsb' (start len : Nat) (x : BitVec n) : BitVec len := .ofNat _ (x.toNat >>> start)
+#check Int.ofNat
+inductive BitField : Nat → Type
+  | ofBitVec {w} : BitVec w → BitField w
+  -- | append {w v} : BitField w → BitField v → BitField (w + v)
+  | cons {v w} : BitField v → BitVec w → BitField (v + w)
+
+namespace BitField
+variable {u v w}
+
+instance : Coe (BitVec w) (BitField w) where
+  coe := ofBitVec
+
+def mk₃ : BitVec u → BitVec v → BitVec w → BitField (u + v + w)
+  | x, y, z => .cons (.cons x y) z
+
+def toBitVec {w} : BitField w → BitVec w
+  | ofBitVec x => x
+  | cons xs x => xs.toBitVec ++ x
+
+def split (xs : BitField (v + w)) : BitVec v × BitVec w :=
+  ⟨xs.toBitVec.extractLsb' w v, xs.toBitVec.extractLsb' 0 w⟩
+
+end BitField
+
+/-
+* https://leanprover-community.github.io/lean4-metaprogramming-book/main/06_macros.html
+* https://leanprover-community.github.io/mathlib4_docs/Init/Prelude.html#Lean.Macro.throwUnsupported
+-/
+
+abbrev BitVec.extract {w} (x : BitVec w) (start len : Nat) (_h : start + len ≤ w) : BitVec len :=
+  x.extractLsb' start len
+
+macro:max x:term noWs kt:"%[" ns:term,* "]" : term =>
+  match ns.getElems.toList with
+  | [] => Lean.Macro.throwErrorAt kt "must have at least 1 element"
+  | m::ns =>
+  let rec genProd : List Lean.Term → Lean.MacroM (Lean.Term × Lean.Term)
+    | [] => return ⟨← ``(BitVec.extractLsb' 0 $m $x), m⟩
+    | n::ns => do
+      let ⟨xs, sum⟩ ← genProd ns
+      return ⟨← ``(Prod.mk (BitVec.extractLsb' $sum $n $x) $xs), ← `($n + $sum)⟩
+  return x
+  -- return (← genProd ns.getElems.toList).1
+
+#check_failure (0#7)%[]
+#check (0#7)%[6]
+example : (0#7)%[7] = 0#7 := rfl
+example : (0#7)%[7] = (0#7) := rfl
+-- example : (0#7)%[3, 4] = (0#3, 0#4) := rfl
+#check (0#7)%[3, 2, 3]  -- FIXME: should fail
